end of day 08/08/19

formal/theory_cleaner.py
@@ -11,41 +11,43 @@ import os
 
 root = '/home/michael/Documents/efsm-inference/'
 
-for root, dirs, files in os.walk(root):
-    for file in files:
-        if file.endswith(".thy"):
-            lemmas_named = set()
-            lemmas_used = set()
-            duplicate_names = set()
-            filepath = os.path.join(root, file)
-            with open(filepath) as f:
-                theory = f.read()
-                named_lemmas = re.finditer('\s*(have|lemma) ((\w)*?):', theory)
-                applies = re.finditer('\s*(apply|by) \((simp|metis|simp_all) (add|only): ((\w|\.|\s*)*)\s*\)\s*', theory)
-                usings = re.finditer('\s*using ((\w| )*)\s*', theory)
-                lemmas = re.finditer('\s*lemmas \w* = ((\w| )*)', theory)
-            for lemma in named_lemmas:
+#for root, dirs, files in os.walk(root):
+#    for file in files:
+root = "inference"
+file = "Can_Take.thy"
+if file.endswith(".thy"):
+    lemmas_named = set()
+    lemmas_used = set()
+    duplicate_names = set()
+    filepath = os.path.join(root, file)
+    with open(filepath) as f:
+        theory = f.read()
+        named_lemmas = re.finditer('\s*(have|lemma) ((\w)*?):', theory)
+        applies = re.finditer('\s*(apply|by) \((simp|metis|simp_all) (add|only): ((\w|\(|\)|_|\.|\s*)*)\s*\)\s*', theory)
+        usings = re.finditer('\s*using ((\w| )*)\s*', theory)
+        lemmas = re.finditer('\s*lemmas \w* = ((\w| )*)', theory)
+    for lemma in named_lemmas:
 #                print(lemma.group(2))
-                if lemma.group(2) in lemmas_named:
-                    duplicate_names.add(lemma.group(2))
-                else:
-                    lemmas_named.add(lemma.group(2))
-            for apply in applies:
+        if lemma.group(2) in lemmas_named:
+            duplicate_names.add(lemma.group(2))
+        else:
+            lemmas_named.add(lemma.group(2))
+    for apply in applies:
 #                print(apply.group(4).split(' '))
-                lemmas_used = lemmas_used.union(set([x.strip() for x in apply.group(4).split(' ')]))
-            for using in usings:
+        lemmas_used = lemmas_used.union(set([x.strip() for x in apply.group(4).split(' ')]))
+    for using in usings:
 #                print(using.group(1).split(' '))
-                lemmas_used = lemmas_used.union(set([x.strip() for x in using.group(1).split(' ')]))
-            for lemma in lemmas:
+        lemmas_used = lemmas_used.union(set([x.strip() for x in using.group(1).split(' ')]))
+    for lemma in lemmas:
 #                print(lemma.group(1).split(' '))
-                lemmas_used = lemmas_used.union([x.strip() for x in set(lemma.group(1).split(' '))])
+        lemmas_used = lemmas_used.union([x.strip() for x in set(lemma.group(1).split(' '))])
 
-            if len(lemmas_named.difference(lemmas_used)) > 0 or len(duplicate_names) > 0:
-                print(file)
-    #            print(len(lemmas_named), sorted(list(lemmas_named)))
-    #            print()
-    #            print(len(lemmas_used.intersection(lemmas_named)), sorted(list(lemmas_used.intersection(lemmas_named))))
-    #            print()
-                print(len(lemmas_named.difference(lemmas_used)), sorted(list(lemmas_named.difference(lemmas_used))))
-                print(sorted(list(duplicate_names)))
-                print('\n')
+    if len(lemmas_named.difference(lemmas_used)) > 0 or len(duplicate_names) > 0:
+        print(file)
+#            print(len(lemmas_named), sorted(list(lemmas_named)))
+#            print()
+#            print(len(lemmas_used.intersection(lemmas_named)), sorted(list(lemmas_used.intersection(lemmas_named))))
+#            print()
+        print(len(lemmas_named.difference(lemmas_used)), sorted(list(lemmas_named.difference(lemmas_used))))
+        print(sorted(list(duplicate_names)))
+        print('\n')
