formal/GExp.thy
@@ -58,6 +58,40 @@ next
     by simp
 qed
 
+lemma gval_gAnd: "gval (gAnd g1 g2) s = (gval g1 s) \<and>\<^sub>? (gval g2 s)"
+proof(induct "gval g1 s" "gval g2 s" rule: times_trilean.induct)
+case 1
+  then show ?case
+    by (metis gval.simps(5) maybe_and_valid maybe_not_invalid maybe_or_invalid)
+next
+  case "2_1"
+  then show ?case
+    by simp
+next
+  case "2_2"
+  then show ?case
+    by simp
+next
+  case 3
+  then show ?case
+    by simp
+next
+  case "4_1"
+  then show ?case
+    by simp
+next
+  case "4_2"
+  then show ?case
+    by simp
+next
+  case 5
+  then show ?case
+    by simp
+qed
+
+lemma gval_gAnd_True: "(gval (gAnd g1 g2) s = true) = ((gval g1 s = true) \<and> gval g2 s = true)"
+  using gval_gAnd maybe_and_not_true by fastforce
+
 abbreviation Lt :: "aexp \<Rightarrow> aexp \<Rightarrow> gexp" (*infix "<" 60*) where
   "Lt a b \<equiv> Gt b a"
 
@@ -87,15 +121,34 @@ lemma nor_equiv: "gval (gNot (gOr a b)) s = gval (Nor a b) s"
 definition satisfiable :: "gexp \<Rightarrow> bool" where
   "satisfiable g \<equiv> (\<exists>i r. gval g (join_ir i r) = true)"
 
+lemma unsatisfiable_false: "\<not> satisfiable (Bc False)"
+  by (simp add: satisfiable_def)
+
 definition "satisfiable_list l = satisfiable (fold gAnd l (Bc True))"
 
 lemma satisfiable_true: "satisfiable (Bc True)"
   by (simp add: satisfiable_def)
 
 definition valid :: "gexp \<Rightarrow> bool" where
-  "valid g \<equiv> (\<forall>i r. gval g (join_ir i r) = true)"
+  "valid g \<equiv> (\<forall>s. gval g s = true)"
+
+lemma valid_true: "valid (Bc True)"
+  by (simp add: valid_def)
 
 definition "valid_list l = valid (fold gAnd l (Bc True))"
+
+lemma valid_list_all_valid: "valid_list G = (\<forall>g \<in> set G. valid g)"
+proof(induct G rule: rev_induct)
+case Nil
+  then show ?case
+    by (simp add: valid_list_def valid_def)
+next
+case (snoc a G)
+  then show ?case
+    apply (simp add: valid_list_def fold_conv_foldr valid_def del: foldr.simps)
+    apply (simp only: foldr.simps comp_def gval_gAnd maybe_and_true)
+    by auto
+qed
 
 definition gexp_equiv :: "gexp \<Rightarrow> gexp \<Rightarrow> bool" where
   "gexp_equiv a b \<equiv> \<forall>s. gval a s = gval b s"
@@ -130,42 +183,6 @@ lemma gAnd_symmetry: "gexp_equiv (gAnd x y) (gAnd y x)"
 lemma satisfiable_gAnd_self: "satisfiable (gAnd x x) = satisfiable x"
   by (simp add: gAnd_reflexivity gexp_equiv_satisfiable)
 
-lemma gval_gAnd: "gval (gAnd g1 g2) s = (gval g1 s) \<and>\<^sub>? (gval g2 s)"
-proof(induct "gval g1 s" "gval g2 s" rule: times_trilean.induct)
-case 1
-  then show ?case
-    by (metis gval.simps(5) maybe_and_valid maybe_not.simps(3) maybe_or_valid)
-next
-  case "2_1"
-  then show ?case
-    by simp
-next
-  case "2_2"
-  then show ?case
-    by simp
-next
-  case 3
-  then show ?case
-    by simp
-next
-  case "4_1"
-  then show ?case
-    by simp
-next
-  case "4_2"
-  then show ?case
-    by simp
-next
-  case 5
-  then show ?case
-    by simp
-qed
-
-lemma gval_gAnd_True: "(gval (gAnd g1 g2) s = true) = ((gval g1 s = true) \<and> gval g2 s = true)"
-  using gval_gAnd maybe_and_not_true by fastforce
-
-declare gval.simps [simp del]
-
 fun gexp_constrains :: "gexp \<Rightarrow> aexp \<Rightarrow> bool" where
   "gexp_constrains (gexp.Bc _) _ = False" |
   "gexp_constrains (Null a) v = aexp_constrains a v" |
@@ -190,7 +207,7 @@ lemma gval_foldr_true: "(gval (foldr gAnd G (Bc True)) s = true) = (\<forall>g \
 proof(induct G)
   case Nil
   then show ?case
-    by (simp add: gval.simps)
+    by simp
 next
   case (Cons a G)
   then show ?case
@@ -251,6 +268,18 @@ qed
 definition max_input :: "gexp \<Rightarrow> nat option" where
   "max_input g = (let inputs = (enumerate_gexp_inputs g) in if inputs = {} then None else Some (Max inputs))"
 
+definition max_input_list :: "gexp list \<Rightarrow> nat option" where
+  "max_input_list g = (fold max (map (\<lambda>g. GExp.max_input g) g) None)"
+
+lemma max_input_list_cons: "max_input_list (a # G) = max (GExp.max_input a) (max_input_list G)"
+  apply (simp add: max_input_list_def)
+proof -
+  have "foldr max (GExp.max_input a # rev (map_tailrec GExp.max_input G)) None = foldr max (rev (None # map_tailrec GExp.max_input G)) (GExp.max_input a)"
+    by (metis (no_types) Max.set_eq_fold comp_def fold.simps(2) fold_conv_foldr foldr_conv_fold list.set(2) max.commute set_rev)
+  then show "fold max (map GExp.max_input G) (max (GExp.max_input a) None) = max (GExp.max_input a) (fold max (map GExp.max_input G) None)"
+    by (simp add: fold_conv_foldr map_eq_map_tailrec max.commute)
+qed
+
 fun enumerate_gexp_regs :: "gexp \<Rightarrow> nat set" where
   "enumerate_gexp_regs (GExp.Bc _) = {}" |
   "enumerate_gexp_regs (GExp.Null v) = enumerate_aexp_regs v" |
@@ -288,6 +317,104 @@ next
     by (simp add: enumerate_aexp_regs_list)
 qed
 
+lemma no_variables_list_gval:
+  "enumerate_gexp_inputs_list g = [] \<Longrightarrow>
+   enumerate_gexp_regs_list g = [] \<Longrightarrow>
+   gval g s = gval g s'"
+proof(induct g)
+case (Bc x)
+  then show ?case
+    by (metis (full_types) gval.simps(1) gval.simps(2))
+next
+  case (Eq x1a x2)
+  then show ?case
+    by (metis append_is_Nil_conv enumerate_gexp_inputs_list.simps(3) enumerate_gexp_regs_list.simps(3) gval.simps(4) no_variables_list_aval)
+next
+  case (Gt x1a x2)
+  then show ?case
+    by (metis Nil_is_append_conv enumerate_gexp_inputs_list.simps(4) enumerate_gexp_regs_list.simps(4) gval.simps(3) no_variables_list_aval)
+next
+  case (Nor a1 a2)
+  then show ?case
+    by simp
+next
+  case (Null x)
+  then show ?case
+    by (metis enumerate_gexp_inputs_list.simps(2) enumerate_gexp_regs_list.simps(2) gval.simps(6) no_variables_list_aval)
+qed
+
+lemma no_variables_list_valid_or_unsat:
+  "enumerate_gexp_inputs_list g = [] \<Longrightarrow>
+   enumerate_gexp_regs_list g = [] \<Longrightarrow>
+   valid g \<or> \<not> satisfiable g"
+proof(induct g)
+case (Bc x)
+  then show ?case
+    apply (cases x)
+     apply (simp add: valid_true)
+    by (simp add: unsatisfiable_false)
+next
+case (Eq x1a x2)
+  then show ?case
+    apply (simp add: valid_def satisfiable_def)
+    by (metis no_variables_list_aval)
+next
+case (Gt x1a x2)
+  then show ?case
+    apply (simp add: valid_def satisfiable_def)
+    by (metis no_variables_list_aval)
+next
+  case (Nor g1 g2)
+  then show ?case
+    apply (simp add: valid_def satisfiable_def)
+    by (metis no_variables_list_gval)
+next
+  case (Null x)
+  then show ?case 
+    apply (simp add: valid_def satisfiable_def)
+    by (metis no_variables_list_aval)
+qed
+
+lemma gval_ir_take: "A \<le> length i \<Longrightarrow>
+      enumerate_gexp_regs_list a = [] \<Longrightarrow>
+      enumerate_gexp_inputs_list a \<noteq> [] \<Longrightarrow>
+      foldr max (enumerate_gexp_inputs_list a) 0 < A \<Longrightarrow>
+      gval a (join_ir (take A i) r) = gval a (join_ir i ra)"
+proof(induct a)
+case (Bc x)
+  then show ?case
+    by simp
+next
+  case (Eq x1a x2)
+  then show ?case
+    apply simp
+    apply (case_tac "enumerate_aexp_inputs_list x1a = []")
+     apply simp
+     apply (metis aval_ir_take no_variables_list_aval)
+    apply simp
+    by (metis Eq.prems(1) Eq.prems(4) List.finite_set Max.set_eq_fold Max_insert aval_ir_take fold_simps(1) foldr_conv_fold list.set(2) max.commute max_0L max_less_iff_conj no_variables_list_aval set_empty set_rev)
+next
+  case (Gt x1a x2)
+  then show ?case
+    apply simp
+    apply (case_tac "enumerate_aexp_inputs_list x1a = []")
+     apply simp
+     apply (metis aval_ir_take no_variables_list_aval)
+    apply simp
+    by (metis List.finite_set Max.set_eq_fold Max_insert aval_ir_take foldr.simps(1) foldr_conv_fold id_apply list.set(2) max_less_iff_conj no_variables_list_aval set_empty set_rev)
+next
+  case (Nor a1 a2)
+  then show ?case
+    apply simp
+    apply clarify
+    by (metis List.finite_set Max.set_eq_fold Max_insert foldr.simps(1) foldr_conv_fold id_apply list.set(2) max_less_iff_conj no_variables_list_gval set_empty set_rev)
+next
+  case (Null x)
+  then show ?case
+    apply simp
+    by (metis aval_ir_take)
+qed
+
 definition max_reg :: "gexp \<Rightarrow> nat option" where
   "max_reg g = (let regs = (enumerate_gexp_regs g) in if regs = {} then None else Some (Max regs))"
 
@@ -313,7 +440,7 @@ lemma no_reg_gval_swap_regs: "GExp.max_reg g = None \<Longrightarrow> gval g (jo
 proof(induct g)
 case (Bc x)
   then show ?case
-    by (metis gval.simps(1) gval.simps(2))
+    by (metis (full_types) gval.simps(1) gval.simps(2))
 next
   case (Eq x1a x2)
   then show ?case
@@ -325,7 +452,7 @@ next
 next
   case (Nor g1 g2)
   then show ?case
-    by (simp add: gval.simps(5) max_is_None max_reg_Nor)
+    by (simp add: max_is_None max_reg_Nor)
 next
   case (Null x)
   then show ?case
@@ -355,7 +482,14 @@ next
     by (simp add: enumerate_aexp_regs_empty_reg_unconstrained)
 qed
 
-lemma enumerate_gexp_inputs_empty_input_unconstrained: "enumerate_gexp_inputs g = {} \<Longrightarrow> \<forall>r. \<not> gexp_constrains g (V (vname.I r))"
+lemma enumerate_gexp_regs_set_reg_unconstrained:
+  "\<forall>x\<in>set G. enumerate_gexp_regs x = {} \<Longrightarrow>
+   \<forall>r. \<forall>g\<in>set G. \<not> gexp_constrains g (V (R r))"
+  by (simp add: enumerate_gexp_regs_empty_reg_unconstrained)
+
+lemma enumerate_gexp_inputs_empty_input_unconstrained:
+  "enumerate_gexp_inputs g = {} \<Longrightarrow>
+   \<forall>r. \<not> gexp_constrains g (V (vname.I r))"
 proof(induct g)
 case (Bc x)
   then show ?case
@@ -378,27 +512,32 @@ next
     by (simp add: enumerate_aexp_inputs_empty_input_unconstrained)
 qed
 
-lemma input_unconstrained_gval_input_swap: "\<forall>r. \<not> gexp_constrains a (V (vname.I r)) \<Longrightarrow> (gval a (join_ir i r) = gval a (join_ir i' r))"
+lemma enumerate_gexp_inputs_set_input_unconstrained:
+  "\<forall>x\<in>set G. enumerate_gexp_inputs x = {} \<Longrightarrow>
+   \<forall>r. \<forall>g\<in>set G. \<not> gexp_constrains g (V (vname.I r))"
+  by (simp add: enumerate_gexp_inputs_empty_input_unconstrained)
+
+lemma input_unconstrained_gval_input_swap:
+  "\<forall>r. \<not> gexp_constrains a (V (vname.I r)) \<Longrightarrow>
+  (gval a (join_ir i r) = gval a (join_ir i' r))"
 proof(induct a)
   case (Bc x)
   then show ?case
-    apply (cases x)
-     apply (simp add: gval.simps(1))
-    by (simp add: gval.simps(2))
+    by (simp add: no_variables_list_gval)
 next
   case (Eq x1a x2)
   then show ?case
-    apply (simp add: gval.simps ValueEq_def)
+    apply (simp add: ValueEq_def)
     by (metis input_unconstrained_aval_input_swap)
 next
   case (Gt x1a x2)
   then show ?case
-    apply (simp add: gval.simps ValueGt_def)
+    apply (simp add: ValueGt_def)
     by (metis input_unconstrained_aval_input_swap)
 next
   case (Nor a1 a2)
   then show ?case
-    by (simp add: gval.simps(5))
+    by simp
 next
   case (Null x)
   then show ?case
@@ -409,23 +548,21 @@ lemma register_unconstrained_gval_register_swap: "\<forall>r. \<not> gexp_constr
 proof(induct a)
   case (Bc x)
   then show ?case
-    apply (cases x)
-     apply (simp add: gval.simps(1))
-    by (simp add: gval.simps(2))
+    by (simp add: no_variables_list_gval)
 next
   case (Eq x1a x2)
   then show ?case
-    apply (simp add: gval.simps ValueEq_def)
+    apply (simp add: ValueEq_def)
     by (metis input_unconstrained_aval_register_swap)
 next
   case (Gt x1a x2)
   then show ?case
-    apply (simp add: gval.simps ValueGt_def)
+    apply (simp add: ValueGt_def)
     by (metis input_unconstrained_aval_register_swap)
 next
   case (Nor a1 a2)
   then show ?case
-    by (simp add: gval.simps(5))
+    by simp
 next
   case (Null x)
   then show ?case
@@ -439,9 +576,7 @@ lemma unconstrained_variable_swap_gval:
 proof(induct g)
 case (Bc x)
   then show ?case
-    apply (cases x)
-     apply (simp add: gval.simps(1))
-    by (simp add: gval.simps(2))
+    by (simp add: no_variables_list_gval)
 next
   case (Eq x1a x2)
   then show ?case
@@ -453,24 +588,30 @@ next
 next
   case (Nor g1 g2)
   then show ?case
-    by (simp add: gval.simps(5))
+    by simp
 next
   case (Null x)
   then show ?case
     by (metis gexp_constrains.simps(2) gval.simps(6) unconstrained_variable_swap_aval)
 qed
 
-lemma "gval (foldr gAnd G (Bc True)) s = foldr (\<and>\<^sub>?) (map (\<lambda>g. gval g s) G) true"
+lemma gval_foldr_map_gval: "gval (foldr gAnd G (Bc True)) s = foldr (\<and>\<^sub>?) (map (\<lambda>g. gval g s) G) true"
 proof(induct G)
   case Nil
   then show ?case
-    by (simp add: gval.simps)
+    by simp
 next
   case (Cons a G)
   then show ?case
     apply (simp only: foldr.simps comp_def gval_gAnd)
     by simp
 qed
+
+lemma gval_In_cons: "gval (In v (a # as)) s = (gval (Eq (V v) (L a)) s \<or>\<^sub>? gval (In v as) s)"
+  apply (cases as)
+   apply (simp add: ValueEq_def)
+  apply (simp add: ValueEq_def)
+  by (metis maybe_double_negation maybe_or_idempotent)
 
 lemma possible_to_be_in: "s \<noteq> [] \<Longrightarrow> satisfiable (In v s)"
 proof(induct s)
@@ -479,17 +620,390 @@ case Nil
 next
   case (Cons a s)
   then show ?case
-    apply (case_tac s)
-     apply (simp add: satisfiable_def gval.simps ValueEq_def)
-     apply (case_tac v)
-      apply (simp add: join_ir_def input2state_exists)
-     apply (simp add: join_ir_def)
-    using input2state_exists apply blast
-    apply (simp add: satisfiable_def gval_gOr)
-    by (metis ValueEq_def gval.simps(4) plus_trilean.simps(4) plus_trilean.simps(5) plus_trilean_commutative)
+    apply (simp add: satisfiable_def gval_In_cons)
+    by (metis In.simps(1) ValueEq_def add.commute gval.simps(2) join_ir_double_exists maybe_or_idempotent plus_trilean.simps(6))
 qed
 
 lemma gAnd_commute: "gval (gAnd a b) s = gval (gAnd b a) s"
   using gval_gAnd times_trilean_commutative by auto
+
+fun null_guard :: "gexp \<Rightarrow> bool" where
+  "null_guard (Null _) = True" |
+  "null_guard (Nor g1 g2) = (null_guard g1 \<or> null_guard g2)" |
+  "null_guard _ = False"
+
+definition max_reg_list :: "gexp list \<Rightarrow> nat option" where
+  "max_reg_list g = (fold max (map (\<lambda>g. GExp.max_reg g) g) None)"
+
+lemma max_reg_list_cons: "max_reg_list (a # G) = max (GExp.max_reg a) (max_reg_list G)"
+  apply (simp add: max_reg_list_def)
+  by (metis (no_types, lifting) List.finite_set Max.insert Max.set_eq_fold fold.simps(1) id_apply list.simps(15) max.assoc set_empty)
+
+lemma max_reg_list_append_singleton: "max_reg_list (as@[bs]) = max (max_reg_list as) (max_reg_list [bs])"
+  apply (simp add: max_reg_list_def)
+  by (metis max.commute max_None_r)
+
+lemma max_reg_list_append: "max_reg_list (as@bs) = max (max_reg_list as) (max_reg_list bs)"
+proof(induct bs rule: rev_induct)
+  case Nil
+  then show ?case
+    by (simp add: max_reg_list_def max_None_r)
+next
+  case (snoc x xs)
+  then show ?case
+    by (metis append_assoc max.assoc max_reg_list_append_singleton)
+qed
+
+definition apply_guards :: "gexp list \<Rightarrow> datastate \<Rightarrow> bool" where
+  "apply_guards G s = (\<forall>g \<in> set (map (\<lambda>g. gval g s) G). g = true)"
+
+lemmas apply_guards = datastate apply_guards_def gval.simps ValueEq_def ValueGt_def
+
+lemma no_reg_apply_guards_swap_regs:
+  "max_reg_list G = None \<Longrightarrow>
+   apply_guards G (join_ir i r) = apply_guards G (join_ir i r')"
+  apply (simp add: apply_guards_def max_reg_list_def)
+  by (metis in_set_conv_decomp max_is_None max_reg_list_append max_reg_list_cons max_reg_list_def no_reg_gval_swap_regs)
+
+lemma apply_guards_singleton: "(apply_guards [g] s) = (gval g s = true)"
+  by (simp add: apply_guards_def)
+
+lemma apply_guards_empty [simp]: "apply_guards [] s"
+  by (simp add: apply_guards_def)
+
+lemma apply_guards_cons: "apply_guards (a # G) c = (gval a c = true \<and> apply_guards G c)"
+  by (simp add: apply_guards_def)
+
+lemma apply_guards_double_cons: "apply_guards (y # x # G) s = (gval (gAnd y x) s = true \<and> apply_guards G s)"
+  using apply_guards_cons gval_gAnd_True by auto
+
+lemma apply_guards_append: "apply_guards (a@a') s = (apply_guards a s \<and> apply_guards a' s)"
+  apply (simp add: apply_guards_def)
+  by auto
+
+lemma apply_guards_foldr: "apply_guards G s = (gval (foldr gAnd G (Bc True)) s = true)"
+proof(induct G)
+  case Nil
+  then show ?case
+    by (simp add: apply_guards_def)
+next
+  case (Cons a G)
+  then show ?case
+    apply (simp only: foldr.simps comp_def)
+    using apply_guards_cons gval_gAnd_True by auto
+qed
+
+lemma apply_guards_rev: "apply_guards G s = apply_guards (rev G) s"
+  by (simp add: apply_guards_def)
+
+lemma rev_apply_guards: "apply_guards (rev G) s = apply_guards G s"
+  by (simp add: apply_guards_def)
+
+lemma apply_guards_fold: "apply_guards G s = (gval (fold gAnd G (Bc True)) s = true)"
+  using apply_guards_rev
+  by (simp add: foldr_conv_fold apply_guards_foldr)
+
+lemma fold_apply_guards: "(gval (fold gAnd G (Bc True)) s = true) = apply_guards G s"
+  by (simp add: apply_guards_fold)
+
+lemma foldr_apply_guards: "(gval (foldr gAnd G (Bc True)) s = true) = apply_guards G s"
+  by (simp add: apply_guards_foldr)
+
+lemma apply_guards_subset: "set g' \<subseteq> set g \<Longrightarrow> apply_guards g c \<longrightarrow> apply_guards g' c"
+proof(induct g)
+  case Nil
+  then show ?case
+    by simp
+next
+  case (Cons a g)
+  then show ?case
+    apply (simp add: apply_guards_def)
+    by auto
+qed
+
+lemma apply_guards_swap: 
+  "apply_guards G (join_ir i r) \<Longrightarrow>
+   \<forall>x\<in>set G. enumerate_gexp_regs x = {} \<Longrightarrow>
+   \<forall>x\<in>set G. enumerate_gexp_inputs x = {} \<Longrightarrow>
+   apply_guards G (join_ir i' r')"
+proof(induct G)
+  case Nil
+  then show ?case
+    by (simp add: apply_guards_def)
+next
+  case (Cons a G)
+  then show ?case
+    apply (simp add: apply_guards_cons)
+    by (metis enumerate_gexp_inputs_list enumerate_gexp_regs_list no_variables_list_gval set_empty)
+qed
+
+lemma valid_list_apply_guards: "valid_list G \<Longrightarrow> apply_guards G s"
+  by (simp add: apply_guards_def valid_list_all_valid valid_def)
+
+lemma apply_guards_rearrange: "x \<in> set G \<Longrightarrow> apply_guards G s = apply_guards (x#G) s"
+  apply (simp add: apply_guards_def)
+  by auto
+
+lemma unconstrained_variable_swap:
+  "\<forall>r. \<forall>g\<in>set G. \<not> gexp_constrains g (V (vname.I r)) \<Longrightarrow>
+   \<forall>r. \<forall>g\<in>set G. \<not> gexp_constrains g (V (R r)) \<Longrightarrow>
+   apply_guards G s = apply_guards G s'"
+proof(induct G)
+  case Nil
+  then show ?case
+    by (simp add: apply_guards_def)
+next
+  case (Cons a G)
+  then show ?case
+    unfolding apply_guards_def
+    apply simp
+    by (metis unconstrained_variable_swap_gval)
+qed
+
+lemma unconstrained_variable_swap_apply_guards:
+  "\<forall>r. \<forall>g\<in>set G. \<not> gexp_constrains g (V (vname.I r)) \<Longrightarrow>
+   \<forall>r. \<forall>g\<in>set G. \<not> gexp_constrains g (V (R r)) \<Longrightarrow>
+   gval (foldr gAnd G (Bc True)) s = true \<Longrightarrow>
+   apply_guards G s'"
+proof(induct G)
+  case Nil
+  then show ?case
+    by (simp add: apply_guards_def)
+next
+  case (Cons a G)
+  then show ?case
+    apply (simp only: foldr.simps comp_def gval_gAnd maybe_and_true apply_guards_cons)
+    apply simp
+    by (metis unconstrained_variable_swap_gval)
+qed
+
+lemma max_lt_val: "max (GExp.max_input a) (max_input_list G) = Some i \<Longrightarrow> (GExp.max_input a) \<le> Some i"
+  by (metis max.cobounded1)
+
+lemma max_input_Bc: "GExp.max_input (Bc x) = None"
+  by (simp add: GExp.max_input_def)
+
+lemma gexp_max_input_nor: "GExp.max_input (Nor g1 g2) = max (GExp.max_input g1) (GExp.max_input g2)"
+  apply (simp add: GExp.max_input_def Let_def)
+  apply safe
+    apply (simp add: max_None_l)
+   apply (simp add: max.commute max_None_l)
+  by (metis List.finite_set Max.union enumerate_gexp_inputs_list max_Some_Some)
+
+lemma max_input_Eq: "GExp.max_input (Eq a1 a2) = max (AExp.max_input a1) (AExp.max_input a2)"
+  apply (simp add: AExp.max_input_def GExp.max_input_def Let_def)
+  apply safe
+    apply (simp add: max_None_l)
+   apply (simp add: max.commute max_None_l)
+  by (metis List.finite_set Max.union enumerate_aexp_inputs_list max_Some_Some)
+
+lemma max_reg_list_Eq: "GExp.max_reg (Eq a1 a2) = max (AExp.max_reg a1) (AExp.max_reg a2)"
+  apply (simp add: AExp.max_reg_def GExp.max_reg_def Let_def)
+  apply safe
+    apply (simp add: max_None_l)
+   apply (simp add: max.commute max_None_l)
+  by (metis List.finite_set Max.union enumerate_aexp_regs_list max_Some_Some)
+
+lemma max_input_Gt: "GExp.max_input (Gt a1 a2) = max (AExp.max_input a1) (AExp.max_input a2)"
+  apply (simp add: AExp.max_input_def GExp.max_input_def Let_def)
+  apply safe
+    apply (simp add: max_None_l)
+   apply (simp add: max.commute max_None_l)
+  by (metis List.finite_set Max.union enumerate_aexp_inputs_list max.commute max_Some_Some)
+
+lemma gexp_max_input_Null: "GExp.max_input (Null x) = AExp.max_input x"
+  by (simp add: AExp.max_input_def GExp.max_input_def)
+
+lemma gval_take: "GExp.max_input g < Some a \<Longrightarrow>
+    gval g (join_ir i r) = gval g (join_ir (take a i) r)"
+proof(induct g)
+case (Bc x)
+  then show ?case
+    by (metis (full_types) gval.simps(1) gval.simps(2))
+next
+  case (Eq x1a x2)
+  then show ?case
+    by (metis aval_take gval.simps(4) max_input_Eq max_less_iff_conj)
+next
+  case (Gt x1a x2)
+  then show ?case
+    by (metis aval_take gval.simps(3) max_input_Gt max_less_iff_conj)
+next
+  case (Nor g1 g2)
+  then show ?case
+    by (simp add: maybe_not_eq gexp_max_input_nor)
+next
+  case (Null x)
+  then show ?case
+    by (metis aval_take gexp_max_input_Null gval.simps(6))
+qed
+
+lemma gval_take_flip: "GExp.max_input g < Some a \<Longrightarrow>
+    gval g (join_ir (take a i) r) = gval g (join_ir i r)"
+  by (metis gval_take)
+
+lemma gval_no_reg_swap_regs:
+  "GExp.max_input g < Some a \<Longrightarrow>
+   GExp.max_reg g = None \<Longrightarrow>
+   gval g (join_ir i ra) = gval g (join_ir (take a i) r)"
+proof(induct g)
+case (Bc x)
+  then show ?case
+    by (metis (full_types) gval.simps(1) gval.simps(2))
+next
+  case (Eq x1a x2)
+  then show ?case
+    by (metis gval_take no_reg_gval_swap_regs)
+next
+  case (Gt x1a x2)
+  then show ?case
+    by (metis gval_take no_reg_gval_swap_regs)
+next
+  case (Nor g1 g2)
+  then show ?case
+    by (simp add: gexp_max_input_nor max_reg_Nor max_is_None)
+next
+  case (Null x)
+  then show ?case
+    by (metis gval_take no_reg_gval_swap_regs)
+qed
+
+lemma max_reg_list_none_set: "(max_reg_list G = None) = (\<forall>g \<in> set G. GExp.max_reg g = None)"
+proof(induct G)
+  case Nil
+  then show ?case
+    by (simp add: max_reg_list_def)
+next
+  case (Cons a G)
+  then show ?case
+    by (simp add: max_reg_list_cons max_is_None)
+qed
+
+lemma gval_fold_gAnd_append_singleton:
+  "gval (fold gAnd (a @ [G]) (Bc True)) s = gval (fold gAnd a (Bc True)) s \<and>\<^sub>? gval G s"
+  apply (simp add: fold_conv_foldr del: foldr.simps)
+  by (simp only: foldr.simps comp_def gval_gAnd times_trilean_commutative)
+
+lemma gval_fold_rev_true:
+  "gval (fold gAnd (rev G) (Bc True)) s = true \<Longrightarrow>
+   gval (fold gAnd G (Bc True)) s = true"
+  by (simp add: fold_conv_foldr gval_foldr_true)
+
+lemma gval_fold_not_invalid_all_valid_contra:
+  "\<exists>g \<in> set G. gval g s = invalid \<Longrightarrow>
+   gval (fold gAnd G (Bc True)) s = invalid"
+proof(induct G rule: rev_induct)
+  case Nil
+  then show ?case
+    by simp
+next
+  case (snoc a G)
+  then show ?case
+    apply (simp only: gval_fold_gAnd_append_singleton)
+    apply simp
+    using maybe_and_valid by blast
+qed
+
+lemma gval_fold_not_invalid_all_valid:
+  "gval (fold gAnd G (Bc True)) s \<noteq> invalid \<Longrightarrow>
+   \<forall>g \<in> set G. gval g s \<noteq> invalid"
+  using gval_fold_not_invalid_all_valid_contra by blast
+
+lemma all_gval_not_false:
+  "(\<forall>g \<in> set G. gval g s \<noteq> false) = (\<forall>g \<in> set G. gval g s = true) \<or> (\<exists>g \<in> set G. gval g s = invalid)"
+  using trilean.exhaust by auto
+
+lemma must_have_one_false_contra:
+  "\<forall>g \<in> set G. gval g s \<noteq> false \<Longrightarrow>
+   gval (fold gAnd G (Bc True)) s \<noteq> false"
+  using all_gval_not_false[of G s]
+  apply simp
+  apply (case_tac "(\<forall>g\<in>set G. gval g s = true)")
+  apply simp
+  try
+
+lemma must_have_one_false:
+  "gval (fold gAnd G (Bc True)) s = false \<Longrightarrow>
+   \<exists>g \<in> set G. gval g s = false"
+  using must_have_one_false_contra by blast
+
+lemma all_valid_fold: "\<forall>g \<in> set G. gval g s \<noteq> invalid \<Longrightarrow> gval (fold gAnd G (Bc True)) s \<noteq> invalid"
+proof(induct G rule: rev_induct)
+  case Nil
+  then show ?case
+    by simp
+next
+  case (snoc a G)
+  then show ?case
+    apply (simp add: fold_conv_foldr del: foldr.simps)
+    apply (simp only: foldr.simps comp_def gval_gAnd)
+    by (simp add: maybe_and_invalid)
+qed
+
+lemma one_false_all_valid_false: "\<exists>g\<in>set G. gval g s = false \<Longrightarrow> \<forall>g\<in>set G. gval g s \<noteq> invalid \<Longrightarrow> gval (fold gAnd G (Bc True)) s = false"
+proof(induct G rule: rev_induct)
+  case Nil
+  then show ?case
+    by simp
+next
+  case (snoc x xs)
+  then show ?case
+    apply (simp add: fold_conv_foldr del: foldr.simps)
+    apply (simp only: foldr.simps comp_def gval_gAnd)
+    apply (case_tac "gval x s = false")
+     apply simp
+     apply (case_tac "gval (foldr gAnd (rev xs) (Bc True)) s")
+       apply simp
+      apply simp
+     apply simp
+    using all_valid_fold
+     apply (simp add: fold_conv_foldr)
+    apply simp
+    by (metis maybe_not.cases times_trilean.simps(5))
+qed
+
+lemma gval_fold_rev_false: "gval (fold gAnd (rev G) (Bc True)) s = false \<Longrightarrow> gval (fold gAnd G (Bc True)) s = false"
+  using must_have_one_false[of "rev G" s]
+        gval_fold_not_invalid_all_valid[of "rev G" s]
+  by (simp add: one_false_all_valid_false)
+
+lemma fold_invalid_means_one_invalid: "gval (fold gAnd G (Bc True)) s = invalid \<Longrightarrow> \<exists>g \<in> set G. gval g s = invalid"
+  using all_valid_fold by blast
+
+lemma gval_fold_rev_invalid: "gval (fold gAnd (rev G) (Bc True)) s = invalid \<Longrightarrow> gval (fold gAnd G (Bc True)) s = invalid"
+  using fold_invalid_means_one_invalid[of "rev G" s]
+  by (simp add: gval_fold_not_invalid_all_valid_contra)
+
+lemma gval_fold_rev_equiv_fold: "gval (fold gAnd (rev G) (Bc True)) s =  gval (fold gAnd G (Bc True)) s"
+  apply (cases "gval (fold gAnd (rev G) (Bc True)) s")
+    apply (simp add: gval_fold_rev_true)
+   apply (simp add: gval_fold_rev_false)
+  by (simp add: gval_fold_rev_invalid)
+
+lemma gval_fold_equiv_fold_rev: "gval (fold gAnd G (Bc True)) s = gval (fold gAnd (rev G) (Bc True)) s"
+  by (simp add: gval_fold_rev_equiv_fold)
+
+lemma gval_fold_gAnd: "gval (fold gAnd G (Bc True)) s = fold (\<and>\<^sub>?) (map (\<lambda>g. gval g s) G) true"
+proof(induct G rule: rev_induct)
+  case Nil
+  then show ?case
+    by simp
+next
+  case (snoc a G)
+  then show ?case
+    apply (simp add: fold_conv_foldr del: foldr.simps)
+    by (simp only: foldr.simps comp_def gval_gAnd)
+qed
+
+lemma gval_fold_equiv_gval_foldr: "gval (fold gAnd G (Bc True)) s = gval (foldr gAnd G (Bc True)) s"
+proof -
+  have "gval (fold gAnd G (Bc True)) s = gval (fold gAnd (rev G) (Bc True)) s"
+    using gval_fold_equiv_fold_rev by force
+then show ?thesis
+by (simp add: foldr_conv_fold)
+qed
+
+lemma gval_foldr_equiv_gval_fold: "gval (foldr gAnd G (Bc True)) s = gval (fold gAnd G (Bc True)) s"
+  by (simp add: gval_fold_equiv_gval_foldr)
 
 end
