formal/inference/Can_Take.thy
@@ -1,153 +1,40 @@
 theory Can_Take
-imports Inference
+imports "../EFSM"
 begin
 
 unbundle finfun_syntax
 
-definition finfun2pairs :: "('a :: linorder) \<Rightarrow>f 'b \<Rightarrow> ('a \<times> 'b) list" where
-  "finfun2pairs f = (let keys = finfun_to_list f in zip keys (map (\<lambda>k. f $ k) keys))"
+primrec padding :: "nat \<Rightarrow> 'a list" where
+  "padding 0 = []" |
+  "padding (Suc m) = (Eps (\<lambda>x. True))#(padding m)"
 
-fun null_guard :: "gexp \<Rightarrow> bool" where
-  "null_guard (Null _) = True" |
-  "null_guard (Nor g1 g2) = (null_guard g1 \<or> null_guard g2)" |
-  "null_guard _ = False"
+definition take_or_pad :: "'a list \<Rightarrow> nat \<Rightarrow> 'a list" where
+  "take_or_pad a n = (if length a \<ge> n then take n a else a@(padding (n-length a)))"
 
-definition max_input :: "gexp list \<Rightarrow> nat option" where
-  "max_input g = (fold max (map (\<lambda>g. GExp.max_input g) g) None)"
-
-lemma max_input_cons: "max_input (a # G) = max (GExp.max_input a) (max_input G)"
-  apply (simp add: max_input_def)
-proof -
-  have "foldr max (GExp.max_input a # rev (map_tailrec GExp.max_input G)) None = foldr max (rev (None # map_tailrec GExp.max_input G)) (GExp.max_input a)"
-    by (metis (no_types) Max.set_eq_fold comp_def fold.simps(2) fold_conv_foldr foldr_conv_fold list.set(2) max.commute set_rev)
-  then show "fold max (map GExp.max_input G) (max (GExp.max_input a) None) = max (GExp.max_input a) (fold max (map GExp.max_input G) None)"
-    by (simp add: fold_conv_foldr map_eq_map_tailrec max.commute)
-qed
-
-definition max_reg :: "gexp list \<Rightarrow> nat option" where
-  "max_reg g = (fold max (map (\<lambda>g. GExp.max_reg g) g) None)"
-
-lemma max_reg_cons: "max_reg (a # G) = max (GExp.max_reg a) (max_reg G)"
-  apply (simp add: max_reg_def)
-  by (metis (no_types, lifting) List.finite_set Max.insert Max.set_eq_fold fold.simps(1) id_apply list.simps(15) max.assoc set_empty)
-
-lemma max_reg_append_singleton: "max_reg (as@[bs]) = max (max_reg as) (max_reg [bs])"
-  apply (simp add: max_reg_def)
-  by (metis max.commute max_None_r)
-
-lemma max_reg_append: "max_reg (as@bs) = max (max_reg as) (max_reg bs)"
-proof(induct bs rule: rev_induct)
-  case Nil
+lemma length_padding: "length (padding n) = n"
+proof(induct n)
+  case 0
   then show ?case
-    by (simp add: Can_Take.max_reg_def max_None_r)
-next
-  case (snoc x xs)
-  then show ?case
-    by (metis append_assoc max.assoc max_reg_append_singleton)
-qed
-
-lemma max_lt_val: "max (GExp.max_input a) (Can_Take.max_input G) = Some i \<Longrightarrow> (GExp.max_input a) \<le> Some i"
-  by (metis max.cobounded1)
-
-lemma Max_set_fold: "l \<noteq> [] \<Longrightarrow> Max (set (l)) = fold max l (hd l)"
-proof(induct l)
-  case Nil
-  then show ?case 
     by simp
 next
-  case (Cons a l)
+  case (Suc n)
   then show ?case
-    using Max.set_eq_fold by auto
+    by simp
 qed
 
-lemma max_union: "x \<noteq> [] \<Longrightarrow> y \<noteq> [] \<Longrightarrow> Max (set x \<union> set y) = max (Max (set x)) (Max (set y))"
-  by (simp add: Max.union)
-
-lemma in_not_empty: "x \<in> s \<Longrightarrow> s \<noteq> {}"
-  by auto
-
-lemma gexp_max_input_nor_aux: "x \<in> set (s1) \<Longrightarrow>
-       Some (Max (set (s1) \<union> set (s2))) \<noteq>
-       max (Some (Max (set (s1)))) (Some (Max (set (s2)))) \<Longrightarrow>
-       xa \<in> set (s2) \<Longrightarrow> False"
-  using in_not_empty[of x "set (s1)"]
-  using in_not_empty[of xa "set (s2)"]
-  apply simp
-  apply (simp add: max_union Max_set_fold)
-  by (metis less_option.simps(4) linorder_not_le max_def)
-
-lemma gexp_max_input_nor: "GExp.max_input (Nor g1 g2) = max (GExp.max_input g1) (GExp.max_input g2)"
-  apply (simp add: GExp.max_input_def Let_def)
-  apply safe
-    apply (simp add: max_None_l)
-   apply (simp add: max.commute max_None_l)
-  using enumerate_gexp_inputs_list gexp_max_input_nor_aux by fastforce
-
-lemma gexp_max_reg_nor: "GExp.max_reg (Nor g1 g2) = max (GExp.max_reg g1) (GExp.max_reg g2)"
-  apply (simp add: GExp.max_reg_def Let_def)
-  apply safe
-    apply (simp add: max_None_l)
-   apply (simp add: max.commute max_None_l)
-  by (metis enumerate_gexp_regs_list gexp_max_input_nor_aux)
-
-lemma max_input_Eq: "GExp.max_input (Eq a1 a2) = max (AExp.max_input a1) (AExp.max_input a2)"
-  apply (simp add: AExp.max_input_def GExp.max_input_def Let_def)
-  apply safe
-    apply (simp add: max_None_l)
-   apply (simp add: max.commute max_None_l)
-  using enumerate_aexp_inputs_list gexp_max_input_nor_aux by fastforce
-
-lemma max_reg_Eq: "GExp.max_reg (Eq a1 a2) = max (AExp.max_reg a1) (AExp.max_reg a2)"
-  apply (simp add: AExp.max_reg_def GExp.max_reg_def Let_def)
-  apply safe
-    apply (simp add: max_None_l)
-   apply (simp add: max.commute max_None_l)
-  by (metis enumerate_aexp_regs_list gexp_max_input_nor_aux)
-
-lemma max_input_Gt: "GExp.max_input (Gt a1 a2) = max (AExp.max_input a1) (AExp.max_input a2)"
-  apply (simp add: AExp.max_input_def GExp.max_input_def Let_def)
-  apply safe
-    apply (simp add: max_None_l)
-   apply (simp add: max.commute max_None_l)
-  by (metis Un_commute enumerate_aexp_inputs_list gexp_max_input_nor_aux)
-
-lemma max_reg_Gt: "GExp.max_reg (Gt a1 a2) = max (AExp.max_reg a1) (AExp.max_reg a2)"
-  apply (simp add: AExp.max_reg_def GExp.max_reg_def Let_def)
-  apply safe
-    apply (simp add: max_None_l)
-   apply (simp add: max.commute max_None_l)
-  by (metis enumerate_aexp_regs_list gexp_max_input_nor_aux inf_sup_aci(5))
-
-lemma max_input_Plus: "AExp.max_input (Plus a1 a2) = max (AExp.max_input a1) (AExp.max_input a2)"
-  apply (simp add: AExp.max_input_def Let_def)
-  apply safe
-    apply (simp add: max_None_l)
-   apply (simp add: max.commute max_None_l)
-  using enumerate_aexp_inputs_list gexp_max_input_nor_aux by fastforce
-
-lemma max_input_Minus: "AExp.max_input (Minus a1 a2) = max (AExp.max_input a1) (AExp.max_input a2)"
-  apply (simp add: AExp.max_input_def Let_def)
-  apply safe
-    apply (simp add: max_None_l)
-   apply (simp add: max.commute max_None_l)
-  using enumerate_aexp_inputs_list gexp_max_input_nor_aux by fastforce
-
-lemma max_reg_Minus: "AExp.max_reg (Minus a1 a2) = max (AExp.max_reg a1) (AExp.max_reg a2)"
-  apply (simp add: AExp.max_reg_def Let_def)
-  apply safe
-    apply (simp add: max_None_l)
-   apply (simp add: max.commute max_None_l)
-  by (metis enumerate_aexp_regs_list gexp_max_input_nor_aux)
-
-lemma max_reg_Plus: "AExp.max_reg (Plus a1 a2) = max (AExp.max_reg a1) (AExp.max_reg a2)"
-  apply (simp add: AExp.max_reg_def Let_def)
-  apply safe
-    apply (simp add: max_None_l)
-   apply (simp add: max.commute max_None_l)
-  by (metis enumerate_aexp_regs_list gexp_max_input_nor_aux)
-
-lemma max_input_I: "AExp.max_input (V (vname.I i)) = Some i"
-  by (simp add: AExp.max_input_def)
+lemma length_take_or_pad: "length (take_or_pad a n) = n"
+proof(induct n)
+  case 0
+  then show ?case
+    by (simp add: take_or_pad_def)
+next
+  case (Suc n)
+  then show ?case
+    apply (simp add: take_or_pad_def)
+    apply standard
+     apply auto[1]
+    by (simp add: length_padding)
+qed
 
 definition ensure_not_null :: "nat \<Rightarrow> gexp list" where
   "ensure_not_null n = map (\<lambda>i. gNot (Null (V (vname.I i)))) [0..<n]"
@@ -166,67 +53,11 @@ next
     apply (simp add: ensure_not_null_def apply_guards_append)
     apply (simp add: apply_guards_singleton maybe_negate_true maybe_or_false)
     apply (case_tac "join_ir ia r (vname.I a) = None")
-     apply simp
+     apply (simp add: ValueEq_def)
     by (simp add: Suc_leI datastate(1) input2state_not_None)
 qed
 
-lemma gexp_max_input_null: "GExp.max_input (Null x) = AExp.max_input x"
-  by (simp add: AExp.max_input_def GExp.max_input_def)
-
-lemma gexp_max_reg_null: "GExp.max_reg (Null x) = AExp.max_reg x"
-  by (simp add: AExp.max_reg_def GExp.max_reg_def)
-
-lemma aval_take: "AExp.max_input x < Some a \<Longrightarrow> aval x (join_ir i r) = aval x (join_ir (take a i) r)"
-proof(induct x)
-  case (L x)
-  then show ?case
-    by simp
-next
-  case (V x)
-  then show ?case
-    apply (cases x)
-    apply (simp add: join_ir_def max_input_I)
-    apply (metis leI nat_less_le take_all test_aux_aux_2)
-    using enumerate_aexp_inputs.simps(3) enumerate_aexp_inputs_empty_input_unconstrained input_unconstrained_aval_input_swap by blast
-next
-  case (Plus x1 x2)
-  then show ?case
-    by (simp add: max_input_Plus)
-next
-  case (Minus x1 x2)
-  then show ?case
-    by (simp add: max_input_Minus)
-qed
-
-lemma gval_take: "GExp.max_input g < Some a \<Longrightarrow>
-    gval g (join_ir i r) = gval g (join_ir (take a i) r)"
-proof(induct g)
-case (Bc x)
-  then show ?case
-    by (metis (full_types) gval.simps(1) gval.simps(2))
-next
-  case (Eq x1a x2)
-  then show ?case
-    by (metis apply_guards(7) aval_take max.strict_boundedE max_input_Eq)
-next
-  case (Gt x1a x2)
-  then show ?case
-    by (metis apply_guards(6) aval_take max.strict_boundedE max_input_Gt)
-next
-  case (Nor g1 g2)
-  then show ?case
-    by (simp add: maybe_not_eq gexp_max_input_nor)
-next
-  case (Null x)
-  then show ?case
-    by (metis apply_guards(9) aval_take gexp_max_input_null)
-qed
-
-lemma gval_take_flip: "GExp.max_input g < Some a \<Longrightarrow>
-    gval g (join_ir (take a i) r) = gval g (join_ir i r)"
-  by (metis gval_take)
-
-lemma apply_guards_take_or_pad: "Can_Take.max_input G < Some a \<Longrightarrow>
+lemma apply_guards_take_or_pad: "max_input_list G < Some a \<Longrightarrow>
        apply_guards G (join_ir i r) \<Longrightarrow>
        apply_guards (ensure_not_null a) (join_ir i r) \<Longrightarrow>
        apply_guards G (join_ir (take_or_pad i a) r)"
@@ -237,15 +68,28 @@ proof(induct G)
 next
   case (Cons g gs)
   then show ?case
-    apply (simp add: apply_guards_cons max_input_cons)
+    apply (simp add: apply_guards_cons max_input_list_cons)
     using not_null_length[of a i r]
     apply simp
     apply (simp add: take_or_pad_def)
     by (metis gval_take)
 qed
 
+(* Begin can take *)
+
+definition can_take :: "nat \<Rightarrow> gexp list \<Rightarrow> inputs \<Rightarrow> registers \<Rightarrow> bool" where
+  "can_take a g i r = (length i = a \<and> apply_guards g (join_ir i r))"
+
+definition "can_take_transition t i r = can_take (Arity t) (Guard t) i r"
+
+lemma can_take_transition_empty_guard: "Guard t = [] \<Longrightarrow> \<exists>i. can_take_transition t i c"
+  by (simp add: can_take_transition_def can_take_def Ex_list_of_length)
+
+lemma valid_list_can_take: "valid_list (Guard t) \<Longrightarrow> \<exists>i. can_take_transition t i c"
+  by (simp add: can_take_transition_def can_take_def valid_list_apply_guards Ex_list_of_length)
+
 lemma satisfiable_can_take:
-  "max_input (Guard t) < Some (Arity t) \<Longrightarrow>
+  "max_input_list (Guard t) < Some (Arity t) \<Longrightarrow>
    satisfiable_list ((Guard t) @ ensure_not_null (Arity t)) \<Longrightarrow>
    \<exists>i r. can_take_transition t i r"
   apply (simp add: can_take_transition_def satisfiable_list_def satisfiable_def fold_apply_guards
@@ -257,62 +101,9 @@ lemma satisfiable_can_take:
   apply (rule_tac x=r in exI)
   by (simp add: apply_guards_take_or_pad)
 
-lemma max_is_none: "(max x y = None) = (x = None \<and> y = None)"
-  by (metis max.commute max_def max_None_l)
-
-lemma aval_no_reg_swap_regs:
-  "AExp.max_input x < Some a \<Longrightarrow>
-   AExp.max_reg x = None \<Longrightarrow>
-   aval x (join_ir i ra) = aval x (join_ir (take a i) r)"
-proof(induct x)
-case (L x)
-  then show ?case
-    by simp
-next
-  case (V x)
-  then show ?case
-    apply (cases x)
-     apply (metis aval_take enumerate_aexp_regs.simps(3) enumerate_aexp_regs_empty_reg_unconstrained input_unconstrained_aval_register_swap)
-    by (simp add: AExp.max_reg_def)
-next
-  case (Plus x1 x2)
-  then show ?case
-    by (simp add: max_input_Plus max_is_none max_reg_Plus)
-next
-  case (Minus x1 x2)
-  then show ?case
-    by (simp add: max_input_Minus max_is_none max_reg_Minus)
-qed
-
-lemma gval_no_reg_swap_regs:
-  "GExp.max_input g < Some a \<Longrightarrow>
-   GExp.max_reg g = None \<Longrightarrow>
-   gval g (join_ir i ra) = gval g (join_ir (take a i) r)"
-proof(induct g)
-case (Bc x)
-  then show ?case
-    by (metis (full_types) gval.simps(1) gval.simps(2))
-next
-  case (Eq x1a x2)
-  then show ?case
-    by (metis apply_guards(7) aval_no_reg_swap_regs max.strict_boundedE max_input_Eq max_is_none max_reg_Eq)
-next
-  case (Gt x1a x2)
-  then show ?case
-    by (metis apply_guards(6) aval_no_reg_swap_regs max.strict_boundedE max_input_Gt max_is_none max_reg_Gt)
-next
-  case (Nor g1 g2)
-  then show ?case
-    by (simp add: gexp_max_input_nor gexp_max_reg_nor max_is_none)
-next
-  case (Null x)
-  then show ?case
-    by (metis apply_guards(9) aval_no_reg_swap_regs gexp_max_input_null gexp_max_reg_null)
-qed
-
 lemma apply_guards_no_reg_swap_regs:
-  "max_reg G = None \<Longrightarrow>
-   max_input G < Some a \<Longrightarrow>
+  "max_reg_list G = None \<Longrightarrow>
+   max_input_list G < Some a \<Longrightarrow>
    apply_guards G (join_ir i ra) \<Longrightarrow>
    apply_guards (ensure_not_null a) (join_ir i ra) \<Longrightarrow>
    apply_guards G (join_ir (take_or_pad i a) r)"
@@ -323,12 +114,12 @@ proof(induct G)
 next
   case (Cons g gs)
   then show ?case
-    by (metis apply_guards_cons gval_no_reg_swap_regs max.strict_boundedE max_input_cons max_is_none max_reg_cons not_null_length take_or_pad_def)
+    by (metis apply_guards_cons gval_no_reg_swap_regs max.strict_boundedE max_input_list_cons max_is_None max_reg_list_cons not_null_length take_or_pad_def)
 qed
 
 lemma can_take_satisfiable:
-  "max_reg (Guard t) = None \<Longrightarrow>
-   max_input (Guard t) < Some (Arity t) \<Longrightarrow>
+  "max_reg_list (Guard t) = None \<Longrightarrow>
+   max_input_list (Guard t) < Some (Arity t) \<Longrightarrow>
    satisfiable_list ((Guard t) @ ensure_not_null (Arity t)) \<Longrightarrow>
    \<exists>i. can_take_transition t i r"
   apply (simp add: can_take_transition_def satisfiable_list_def satisfiable_def fold_apply_guards
@@ -339,65 +130,15 @@ lemma can_take_satisfiable:
    apply (simp add: length_take_or_pad)
   by (simp add: apply_guards_no_reg_swap_regs)
 
-definition simple_mutex :: "transition \<Rightarrow> transition \<Rightarrow> bool" where
-  "simple_mutex t t' = (max_reg (Guard t) = None \<and>
-     max_input (Guard t) < Some (Arity t) \<and>
-     satisfiable_list ((Guard t) @ ensure_not_null (Arity t)) \<and>
-     Label t = Label t' \<and>
-     Arity t = Arity t' \<and>
-     \<not> choice t' t)"
-
-lemma simple_mutex_direct_subsumption:
-  "simple_mutex t t' \<Longrightarrow>
-   \<not> directly_subsumes e e' s s' t' t"
-  apply (rule cant_directly_subsume)
-  apply (rule allI)
-  apply (simp add: simple_mutex_def)
-  by (metis can_take_satisfiable no_choice_no_subsumption)
-
-(*
-lemma apply_guards_no_reg_swap_regs:
-  "max_reg G = None \<Longrightarrow>
-   max_input G < Some a \<Longrightarrow>
-   apply_guards G (join_ir i ra) \<Longrightarrow>
-   apply_guards (ensure_not_null a) (join_ir i ra) \<Longrightarrow>
-   apply_guards G (join_ir (take_or_pad i a) r)"
-proof(induct G)
-  case Nil
-  then show ?case
-    by (simp add: max_input_def)
-next
-  case (Cons g gs)
-  then show ?case
-    by (metis apply_guards_cons gval_no_reg_swap_regs max.strict_boundedE max_input_cons
-              max_is_none max_reg_cons not_null_length take_or_pad_def)
-qed
-*)
-
-lemma max_reg_none_set: "(max_reg G = None) = (\<forall>g \<in> set G. GExp.max_reg g = None)"
-proof(induct G)
-  case Nil
-  then show ?case
-    by (simp add: max_reg_def)
-next
-  case (Cons a G)
-  then show ?case
-    by (simp add: max_reg_cons max_is_None)
-qed
-
-lemma no_reg_apply_guards_swap_regs: "max_reg G = None \<Longrightarrow> apply_guards G (join_ir i r) = apply_guards G (join_ir i r')"
-  apply (simp add: apply_guards_def max_reg_none_set)
-  by (metis no_reg_gval_swap_regs)
-
-lemma max_reg_ensure_not_null: "max_reg (ensure_not_null a) = None"
+lemma max_reg_list_ensure_not_null: "max_reg_list (ensure_not_null a) = None"
 proof(induct a)
   case 0
   then show ?case
-    by (simp add: ensure_not_null_def max_reg_def)
+    by (simp add: ensure_not_null_def max_reg_list_def)
 next
   case (Suc a)
   then show ?case
-    by (simp add: ensure_not_null_cons max_reg_append max_reg_def max_reg_gNot max_reg_Null max_reg_V)
+    by (simp add: ensure_not_null_cons max_reg_list_append max_reg_list_def max_reg_gNot max_reg_Null max_reg_V)
 qed
 
 fun not_null :: "gexp \<Rightarrow> bool" where
@@ -405,7 +146,9 @@ fun not_null :: "gexp \<Rightarrow> bool" where
   "not_null (Nor x y) = (not_null x \<and> not_null y)" |
   "not_null _ = True"
 
-lemma apply_guards_ensure_not_null: "length i \<ge> a \<Longrightarrow> apply_guards (ensure_not_null a) (join_ir i r)"
+lemma apply_guards_ensure_not_null:
+  "length i \<ge> a \<Longrightarrow>
+   apply_guards (ensure_not_null a) (join_ir i r)"
 proof(induct a)
   case 0
   then show ?case
@@ -413,210 +156,15 @@ proof(induct a)
 next
   case (Suc a)
   then show ?case
-    apply (simp add: ensure_not_null_cons apply_guards_append apply_guards_singleton)
+    apply (simp add: ensure_not_null_cons apply_guards_append apply_guards_singleton ValueEq_def)
     by (simp add: join_ir_def input2state_nth)
 qed
-
-lemma apply_guards_pad: "apply_guards (ensure_not_null a) (join_ir (padding a) <>)"
-proof(induct a)
-  case 0
-  then show ?case
-    by (simp add: ensure_not_null_def)
-next
-  case (Suc a)
-  then show ?case
-    apply (simp add: ensure_not_null_cons apply_guards_append)
-    apply standard
-     apply (rule apply_guards_ensure_not_null)
-     apply (simp add: length_padding)
-    apply (simp add: apply_guards_singleton join_ir_def)
-    by (metis input2state_nth le_imp_less_Suc length_padding linorder_not_le nat_less_le padding.simps(2))
-qed
-
-lemma max_input_Bc: "GExp.max_input (Bc x) = None"
-  by (simp add: GExp.max_input_def)
-
-lemma Some_lt_max: "Some a \<le> max (AExp.max_input A1) (AExp.max_input A2) \<Longrightarrow>
-       Some a \<le> (AExp.max_input A1) \<or> Some a \<le> (AExp.max_input A2)"
-  by linarith
 
 lemma apply_guards_ensure_not_null_length: "apply_guards (ensure_not_null a) (join_ir i r) = (length i \<ge> a)"
   using apply_guards_ensure_not_null not_null_length by blast
 
-lemma max_input_must_be_some: "(Some a \<le> AExp.max_input A ) \<Longrightarrow> (\<exists>a'. AExp.max_input A = Some a')"
-  using not_le by fastforce
-
-lemma need_aval_I_contra:
-  "\<nexists>n'. aval (V (I a)) (join_ir i r) = Some (Num n') \<Longrightarrow>
-   AExp.max_input A = Some a \<Longrightarrow>
-   \<nexists>n. aval A (join_ir i r) = Some (Num n)"
-proof(induct A)
-  case (L x)
-  then show ?case
-    by (simp add: AExp.max_input_def)
-next
-  case (V x)
-  then show ?case
-    apply (cases x)
-     defer
-     apply (simp add: AExp.max_input_def)
-    by (simp add: join_ir_def max_input_I)
-next
-case (Plus A1 A2)
-  then show ?case
-    apply (simp add: max_input_Plus value_plus_def MaybeArithInt_Not_Num MaybeArithInt_None)
-    by (metis max_def_raw)
-next
-  case (Minus A1 A2)
-  then show ?case
-    apply (simp add: max_input_Minus value_minus_def MaybeArithInt_Not_Num MaybeArithInt_None)
-    by (metis max_def_raw)
-qed
-
-lemma need_aval_I:
-  "AExp.max_input A = Some a \<Longrightarrow>
-   aval A (join_ir i r) = Some (Num n) \<Longrightarrow>
-   \<exists>n'. aval (V (I a)) (join_ir i r) = Some (Num n')"
-  using need_aval_I_contra by blast
-
-lemma aval_input2state_within_bounds: "\<exists>n'. aval (V (I a)) (join_ir i r) = Some (Num n') \<Longrightarrow> a \<le> length i"
-  apply (simp add: join_ir_def)
-  using input2state_within_bounds less_imp_le_nat by blast
-
-lemma aval_Num_apply_guards_not_null:
-"Some a \<le> AExp.max_input A \<Longrightarrow>
- aval A (join_ir i r) = Some (Num n) \<Longrightarrow>
- apply_guards (ensure_not_null a) (join_ir i r)"
-  using max_input_must_be_some[of a A]
-  apply (simp add: apply_guards_ensure_not_null_length)
-  apply clarify
-  using need_aval_I aval_input2state_within_bounds
-  using leD by fastforce
-
 definition negate :: "gexp list \<Rightarrow> gexp" where
   "negate g = gNot (fold gAnd g (Bc True))"
-
-lemma "\<not>\<^sub>? a \<or>\<^sub>? b = \<not>\<^sub>? (a \<or>\<^sub>? b)"
-  by simp
-
-lemma gval_fold_gAnd_append_singleton: "gval (fold gAnd (a @ [G]) (Bc True)) s = gval (fold gAnd a (Bc True)) s \<and>\<^sub>? gval G s "
-  apply (simp add: fold_conv_foldr del: foldr.simps)
-  by (simp only: foldr.simps comp_def gval_gAnd times_trilean_commutative)
-
-lemma gval_fold_rev_true: "gval (fold gAnd (rev G) (Bc True)) s = true \<Longrightarrow> gval (fold gAnd G (Bc True)) s = true"
-  by (simp add: fold_apply_guards apply_guards_def)
-
-lemma gval_fold_not_invalid_all_valid_contra:
-  "\<exists>g \<in> set G. gval g s = invalid \<Longrightarrow> gval (fold gAnd G (Bc True)) s = invalid"
-proof(induct G rule: rev_induct)
-  case Nil
-  then show ?case
-    by simp
-next
-  case (snoc a G)
-  then show ?case
-    apply (simp only: gval_fold_gAnd_append_singleton)
-    apply simp
-    using maybe_and_valid by blast
-qed
-
-lemma gval_fold_not_invalid_all_valid: "gval (fold gAnd G (Bc True)) s \<noteq> invalid \<Longrightarrow> \<forall>g \<in> set G. gval g s \<noteq> invalid"
-  using gval_fold_not_invalid_all_valid_contra by blast
-
-lemma all_gval_not_false: "(\<forall>g \<in> set G. gval g s \<noteq> false) = (\<forall>g \<in> set G. gval g s = true) \<or> (\<exists>g \<in> set G. gval g s = invalid)"
-  using trilean.exhaust by auto
-
-lemma must_have_one_false_contra: "\<forall>g \<in> set G. gval g s \<noteq> false \<Longrightarrow> gval (fold gAnd G (Bc True)) s \<noteq> false"
-  using all_gval_not_false[of G s]
-  apply simp
-  apply (case_tac "(\<forall>g\<in>set G. gval g s = true)")
-  using apply_guards_fold apply_guards_foldr gval_foldr_true apply auto[1]
-  by (simp add: gval_fold_not_invalid_all_valid_contra)
-
-lemma must_have_one_false: "gval (fold gAnd G (Bc True)) s = false \<Longrightarrow> \<exists>g \<in> set G. gval g s = false"
-  using must_have_one_false_contra by blast
-
-lemma all_valid_must_be_true_or_false: "(\<forall>g \<in> set G. gval g s \<noteq> invalid) = (\<forall>g \<in> set G. gval g s = true) \<or> (\<exists>g \<in> set G. gval g s = false)"
-  using all_gval_not_false by auto
-
-lemma all_valid_fold: "\<forall>g \<in> set G. gval g s \<noteq> invalid \<Longrightarrow> gval (fold gAnd G (Bc True)) s \<noteq> invalid"
-proof(induct G rule: rev_induct)
-  case Nil
-  then show ?case
-    by simp
-next
-  case (snoc a G)
-  then show ?case
-    apply (simp add: fold_conv_foldr del: foldr.simps)
-    apply (simp only: foldr.simps comp_def gval_gAnd)
-    by (simp add: maybe_and_invalid)
-qed
-
-lemma one_false_all_valid_false: "\<exists>g\<in>set G. gval g s = false \<Longrightarrow> \<forall>g\<in>set G. gval g s \<noteq> invalid \<Longrightarrow> gval (fold gAnd G (Bc True)) s = false"
-proof(induct G rule: rev_induct)
-  case Nil
-  then show ?case
-    by simp
-next
-  case (snoc x xs)
-  then show ?case
-    apply (simp add: fold_conv_foldr del: foldr.simps)
-    apply (simp only: foldr.simps comp_def gval_gAnd)
-    apply (case_tac "gval x s = false")
-     apply simp
-     apply (case_tac "gval (foldr gAnd (rev xs) (Bc True)) s")
-       apply simp
-      apply simp
-     apply simp
-    using all_valid_fold
-     apply (simp add: fold_conv_foldr)
-    apply simp
-    by (metis maybe_not.cases times_trilean.simps(5))
-qed
-
-lemma gval_fold_rev_false: "gval (fold gAnd (rev G) (Bc True)) s = false \<Longrightarrow> gval (fold gAnd G (Bc True)) s = false"
-  using must_have_one_false[of "rev G" s]
-        gval_fold_not_invalid_all_valid[of "rev G" s]
-  by (simp add: one_false_all_valid_false)
-
-lemma fold_invalid_means_one_invalid: "gval (fold gAnd G (Bc True)) s = invalid \<Longrightarrow> \<exists>g \<in> set G. gval g s = invalid"
-  using all_valid_fold by blast
-
-lemma gval_fold_rev_invalid: "gval (fold gAnd (rev G) (Bc True)) s = invalid \<Longrightarrow> gval (fold gAnd G (Bc True)) s = invalid"
-  using fold_invalid_means_one_invalid[of "rev G" s]
-  by (simp add: gval_fold_not_invalid_all_valid_contra)
-
-lemma gval_fold_rev_equiv_fold: "gval (fold gAnd (rev G) (Bc True)) s =  gval (fold gAnd G (Bc True)) s"
-  apply (cases "gval (fold gAnd (rev G) (Bc True)) s")
-    apply (simp add: gval_fold_rev_true)
-   apply (simp add: gval_fold_rev_false)
-  by (simp add: gval_fold_rev_invalid)
-
-lemma gval_fold_equiv_fold_rev: "gval (fold gAnd G (Bc True)) s = gval (fold gAnd (rev G) (Bc True)) s"
-  by (simp add: gval_fold_rev_equiv_fold)
-
-lemma gval_fold_gAnd: "gval (fold gAnd G (Bc True)) s = fold (\<and>\<^sub>?) (map (\<lambda>g. gval g s) G) true"
-proof(induct G rule: rev_induct)
-  case Nil
-  then show ?case
-    by simp
-next
-  case (snoc a G)
-  then show ?case
-    apply (simp add: fold_conv_foldr del: foldr.simps)
-    by (simp only: foldr.simps comp_def gval_gAnd)
-qed
-
-lemma gval_fold_equiv_gval_foldr: "gval (fold gAnd G (Bc True)) s = gval (foldr gAnd G (Bc True)) s"
-proof -
-  have "gval (fold gAnd G (Bc True)) s = gval (fold gAnd (rev G) (Bc True)) s"
-    using gval_fold_equiv_fold_rev by force
-then show ?thesis
-by (simp add: foldr_conv_fold)
-qed
-
-lemma gval_foldr_equiv_gval_fold: "gval (foldr gAnd G (Bc True)) s = gval (fold gAnd G (Bc True)) s"
-  by (simp add: gval_fold_equiv_gval_foldr)
 
 lemma gval_negate_cons: "gval (negate (a # G)) s = gval (gNot a) s \<or>\<^sub>? gval (negate G) s"
   apply (simp only: negate_def gval_gNot gval_fold_equiv_gval_foldr)
@@ -637,7 +185,7 @@ lemma maybe_or_true_not_invalid: "(true \<or>\<^sub>? x = true) = (x \<noteq> in
 lemma gval_negate_not_invalid: "(gval (negate gs) (join_ir i ra) \<noteq> invalid) = (gval (fold gAnd gs (Bc True)) (join_ir i ra) \<noteq> invalid)"
   using gval_gNot maybe_not_invalid negate_def by auto
 
-lemma gval_fold_swap_regs: "max_reg G = None \<Longrightarrow> gval (fold gAnd G (Bc True)) (join_ir i r) = gval (fold gAnd G (Bc True)) (join_ir i r')"
+lemma gval_fold_swap_regs: "max_reg_list G = None \<Longrightarrow> gval (fold gAnd G (Bc True)) (join_ir i r) = gval (fold gAnd G (Bc True)) (join_ir i r')"
 proof(induct G)
   case Nil
   then show ?case
@@ -646,7 +194,7 @@ next
   case (Cons a G)
   then show ?case
     apply (simp only: gval_fold_equiv_gval_foldr foldr.simps comp_def gval_gAnd)
-    by (metis (no_types, lifting) max_is_None max_reg_cons no_reg_gval_swap_regs)
+    by (metis (no_types, lifting) max_is_None max_reg_list_cons no_reg_gval_swap_regs)
 qed
 
 lemma negate_valid: "(\<not>\<^sub>? x \<noteq> invalid) = (x \<noteq> invalid)"
@@ -665,13 +213,13 @@ lemma maybe_and_not_invalid: "(x \<and>\<^sub>? y \<noteq> invalid) = (x \<noteq
 lemma negate_not_apply_guards: "gval (negate G) s = true \<Longrightarrow> \<not> apply_guards G s"
   by (simp add: apply_guards_fold negate_true_guard)
 
-lemma less_eq_length_trans: "max_input G < Some a \<Longrightarrow> a \<le> length i \<Longrightarrow> max_input G \<le> Some (length i)"
+lemma less_eq_length_trans: "max_input_list G < Some a \<Longrightarrow> a \<le> length i \<Longrightarrow> max_input_list G \<le> Some (length i)"
   by (meson leD less_option.simps(4) not_le_imp_less order.strict_trans)
 
 lemma gval_fold_take:
-  "Can_Take.max_input G < Some a \<Longrightarrow>
+  "max_input_list G < Some a \<Longrightarrow>
    a \<le> length i \<Longrightarrow>
-   Can_Take.max_input G \<le> Some (length i) \<Longrightarrow>
+   max_input_list G \<le> Some (length i) \<Longrightarrow>
    gval (fold gAnd G (Bc True)) (join_ir i r) = gval (fold gAnd G (Bc True)) (join_ir (take a i) r)"
 proof(induct G)
   case Nil
@@ -681,15 +229,14 @@ next
   case (Cons g gs)
   then show ?case
     apply (simp only: gval_fold_cons)
-    apply (simp add: max_input_cons)
+    apply (simp add: max_input_list_cons)
     using gval_take[of g a i r]
     by simp
 qed
 
-
 lemma gval_fold_take_false_not_true:
-  "Can_Take.max_reg G = None \<Longrightarrow>
-   Can_Take.max_input G < Some a \<Longrightarrow>
+  "max_reg_list G = None \<Longrightarrow>
+   max_input_list G < Some a \<Longrightarrow>
    gval (fold gAnd G (Bc True)) (join_ir i ra) = false \<Longrightarrow>
    a \<le> length i \<Longrightarrow>
    gval (fold gAnd G (Bc True)) (join_ir (take a i) r) \<noteq> true"
@@ -697,8 +244,8 @@ lemma gval_fold_take_false_not_true:
   apply (simp add: gval_fold_swap_regs[of G i ra r])
   by (simp add: gval_fold_take)
 
-lemma quick_negation_aux: "Can_Take.max_reg G = None \<Longrightarrow>
-    Can_Take.max_input G < Some a \<Longrightarrow>
+lemma quick_negation_aux: "max_reg_list G = None \<Longrightarrow>
+    max_input_list G < Some a \<Longrightarrow>
     \<exists>i r. gval (negate G) (join_ir i r) = true \<and> apply_guards (ensure_not_null a) (join_ir i r) \<Longrightarrow>
     \<exists>i. length i = a \<and> \<not> apply_guards G (join_ir i r)"
   apply clarify
@@ -709,15 +256,15 @@ lemma quick_negation_aux: "Can_Take.max_reg G = None \<Longrightarrow>
   by (simp add: gval_fold_take_false_not_true)
 
 lemma quick_negation:
-  "max_reg (Guard t) = None \<Longrightarrow>
-   max_input (Guard t) < Some (Arity t) \<Longrightarrow>
+  "max_reg_list (Guard t) = None \<Longrightarrow>
+   max_input_list (Guard t) < Some (Arity t) \<Longrightarrow>
    satisfiable_list (negate (Guard t) # ensure_not_null (Arity t)) \<Longrightarrow>
    \<exists>i. length i = Arity t \<and> \<not> apply_guards (Guard t) (join_ir i r)"
   apply (simp add: satisfiable_list_def satisfiable_def fold_apply_guards apply_guards_cons del: fold.simps)
   by (simp add: quick_negation_aux)
 
-definition "satisfiable_negation t = (max_reg (Guard t) = None \<and>
-   max_input (Guard t) < Some (Arity t) \<and>
+definition "satisfiable_negation t = (max_reg_list (Guard t) = None \<and>
+   max_input_list (Guard t) < Some (Arity t) \<and>
    satisfiable_list (negate (Guard t) # ensure_not_null (Arity t)))"
 
 end
